Phi_System/PhiSem/PhiSem_Min.thy
@@ -13,16 +13,21 @@ subsection \<open>Models\<close>
 subsubsection \<open>Type\<close>
 
 virtual_datatype \<phi>min_ty = \<phi>empty_ty +
-  T_int     :: nat \<comment> \<open>in unit of bits\<close>
+  int     :: nat \<comment> \<open>in unit of bits\<close>
 
 context \<phi>min_ty begin
-abbreviation \<open>\<tau>Int \<equiv> T_int.mk\<close>
+abbreviation int where \<open>int \<equiv> int.mk\<close>
 end
 
 subsubsection \<open>Value\<close>
 
 virtual_datatype 'TY \<phi>min_val :: "nonsepable_semigroup" = 'TY \<phi>empty_val +
-  V_int     :: \<open>nat \<times> nat\<close> \<comment> \<open>bits \<times> value\<close>
+  Int     :: \<open>nat \<times> nat\<close> \<comment> \<open>bits \<times> value\<close>
+
+context \<phi>min_val
+begin
+term int
+end
 
 subsubsection \<open>Resource\<close>
 
@@ -43,11 +48,11 @@ locale \<phi>min_sem =
 + \<phi>min_ty  where CONS_OF   = TY_CONS_OF
             and TYPE'NAME = \<open>TYPE('TY_N)\<close>
             and TYPE'REP  = \<open>TYPE('TY)\<close>
-+ \<phi>min_val where CONS_OF   = VAL_CONS_OF
++ V: \<phi>min_val where CONS_OF   = VAL_CONS_OF
             and TYPE'TY   = \<open>TYPE('TY)\<close>
             and TYPE'NAME = \<open>TYPE('VAL_N)\<close>
             and TYPE'REP  = \<open>TYPE('VAL::nonsepable_semigroup)\<close>
-+ \<phi>min_res where TYPE'VAL  = \<open>TYPE('VAL)\<close>
++ R: \<phi>min_res where TYPE'VAL  = \<open>TYPE('VAL)\<close>
             and TYPE'TY   = \<open>TYPE('TY)\<close>
             and TYPE'NAME = \<open>TYPE('RES_N)\<close>
             and TYPE'REP  = \<open>TYPE('RES::sep_algebra)\<close>
@@ -56,16 +61,16 @@ for TYPES :: \<open>(('TY_N \<Rightarrow> 'TY)
                 \<times> ('VAL_N => 'VAL::nonsepable_semigroup)
                 \<times> ('RES_N => 'RES::sep_algebra)) itself\<close>
 +
-assumes WT_int[simp]: \<open>Well_Type (\<tau>Int b)     = { V_int.mk (b,x)    |x. x < 2 ^ Big b } \<close>
-assumes res_valid_var[simp]: \<open>Resource_Validator R_var.name = {R_var.inject vars |vars. finite (dom vars)}\<close>
-assumes can_eqcmp_int[simp]: "Can_EqCompare res (V_int.mk (b1,x1)) (V_int.mk (b2,x2)) \<longleftrightarrow> b1 = b2"
-assumes eqcmp_int[simp]: "EqCompare (V_int.mk i1) (V_int.mk i2) \<longleftrightarrow> i1 = i2"
-assumes zero_int[simp]: \<open>Zero (T_int.mk b)    = Some (V_int.mk (b,0))\<close>
+assumes WT_int[simp]: \<open>Well_Type (int b)     = { V.Int.mk (b,x)    |x. x < 2 ^ Big b } \<close>
+assumes res_valid_var[simp]: \<open>Resource_Validator R.R_var.name = {R.R_var.inject vars |vars. finite (dom vars)}\<close>
+assumes can_eqcmp_int[simp]: "Can_EqCompare res (V.Int.mk (b1,x1)) (V.Int.mk (b2,x2)) \<longleftrightarrow> b1 = b2"
+assumes eqcmp_int[simp]: "EqCompare (V.Int.mk i1) (V.Int.mk i2) \<longleftrightarrow> i1 = i2"
+assumes zero_int[simp]: \<open>Zero (int b)    = Some (V.Int.mk (b,0))\<close>
 
 begin
 
 lemma Valid_Types[simp]:
-  \<open>Valid_Type (\<tau>Int n)\<close>
+  \<open>Valid_Type (int n)\<close>
   unfolding Inhabited_def
   apply simp
   using less_exp by blast
@@ -79,7 +84,9 @@ fiction_space (in \<phi>min_sem) \<phi>min_fic :: \<open>'RES_N \<Rightarrow> 'R
   FIC_var :: \<open>R_var.raw_basic_fiction \<F>_it\<close>
 
 locale \<phi>min =
-  \<phi>min_fic where TYPES = \<open>TYPE(('TY_N \<Rightarrow> 'TY) \<times> ('VAL_N \<Rightarrow> 'VAL::nonsepable_semigroup)
+  \<phi>min_sem where TYPES = \<open>TYPE(('TY_N \<Rightarrow> 'TY) \<times> ('VAL_N \<Rightarrow> 'VAL::nonsepable_semigroup)
+                            \<times> ('RES_N \<Rightarrow> 'RES::sep_algebra))\<close>
++ F: \<phi>min_fic where TYPES = \<open>TYPE(('TY_N \<Rightarrow> 'TY) \<times> ('VAL_N \<Rightarrow> 'VAL::nonsepable_semigroup)
                             \<times> ('RES_N \<Rightarrow> 'RES::sep_algebra))\<close>
     and TYPE'FNAME = \<open>TYPE('FIC_N)\<close>
     and TYPE'FREP = \<open>TYPE('FIC::sep_algebra)\<close> 
@@ -95,25 +102,26 @@ sublocale FIC_var: identity_fiction \<open>{vars. finite (dom vars)}\<close> R_v
 
 end
 
+
 section \<open>\<phi>-Types\<close>
+
+\<phi>overloads nat and int
 
 context \<phi>min_sem begin
 
 subsection \<open>Integer\<close>
-
-\<phi>overloads nat and int
 
 subsubsection \<open>Natural Nmbers\<close>
 
 paragraph \<open>Natural Number\<close>
 
 definition \<phi>Nat :: "nat \<Rightarrow> ('VAL, nat) \<phi>" ("\<nat>[_]")
-  where "\<nat>[b] x = (if x < 2^b then { V_int.mk (b,x) } else {})"
+  where "\<nat>[b] x = (if x < 2^b then { V.Int.mk (b,x) } else {})"
 
 (* abbreviation \<open>Size \<equiv> \<nat>[addrspace_bits]\<close> *)
 
 lemma \<phi>Nat_expn[\<phi>expns]:
-  "p \<in> (x \<Ztypecolon> \<nat>[b]) \<longleftrightarrow> (p = V_int.mk (b,x)) \<and> x < 2 ^ Big b"
+  "p \<in> (x \<Ztypecolon> \<nat>[b]) \<longleftrightarrow> (p = V.Int.mk (b,x)) \<and> x < 2 ^ Big b"
   unfolding \<phi>Type_def Big_def by (simp add: \<phi>Nat_def)
 
 lemma \<phi>Nat_elim[elim!,\<phi>inhabitance_rule]:
@@ -125,15 +133,15 @@ lemma
   unfolding Inhabited_def by (simp add: \<phi>expns)
 
 lemma \<phi>Nat_semty[\<phi>reason for \<open>\<phi>SemType (?x \<Ztypecolon> \<nat>[?b]) ?ty\<close>]:
-  \<open>\<phi>SemType (x \<Ztypecolon> \<nat>[b]) (\<tau>Int b)\<close>
+  \<open>\<phi>SemType (x \<Ztypecolon> \<nat>[b]) (int b)\<close>
   unfolding \<phi>SemType_def subset_iff by (simp add: \<phi>expns Big_def)
 
 lemma [\<phi>reason for \<open>\<phi>Equal (\<nat>[?b]) ?c ?eq\<close>]:
   "\<phi>Equal (\<nat>[b]) (\<lambda>x y. True) (=)"
   unfolding \<phi>Equal_def by (auto simp add: \<phi>expns)
 
-lemma [\<phi>reason for \<open>\<phi>Zero (T_int.mk ?b) (\<nat>[?b]) ?zero\<close>]:
-  "\<phi>Zero (T_int.mk b) (\<nat>[b]) 0" unfolding \<phi>Zero_def by (simp add: \<phi>expns)
+lemma [\<phi>reason for \<open>\<phi>Zero (int ?b) (\<nat>[?b]) ?zero\<close>]:
+  "\<phi>Zero (int b) (\<nat>[b]) 0" unfolding \<phi>Zero_def by (simp add: \<phi>expns)
 
 lemma [\<phi>reason]:
   \<open> \<^bold>p\<^bold>r\<^bold>e\<^bold>m\<^bold>i\<^bold>s\<^bold>e x < 2^Big b
@@ -143,22 +151,22 @@ lemma [\<phi>reason]:
 paragraph \<open>Rounded Natural Number\<close>
 
 definition \<phi>NatRound :: "nat \<Rightarrow> ('VAL, nat) \<phi>" ("\<nat>\<^sup>r[_]")
-  where "\<nat>\<^sup>r[b] x = { V_int.mk (b, (x mod 2 ^ Big b)) }"
+  where "\<nat>\<^sup>r[b] x = { V.Int.mk (b, (x mod 2 ^ Big b)) }"
 
 lemma \<phi>NatRound_expn[\<phi>expns]:
-  "p \<in> (x \<Ztypecolon> \<nat>\<^sup>r[b]) \<longleftrightarrow> p = V_int.mk (b, (x mod 2 ^ Big b))"
+  "p \<in> (x \<Ztypecolon> \<nat>\<^sup>r[b]) \<longleftrightarrow> p = V.Int.mk (b, (x mod 2 ^ Big b))"
   unfolding \<phi>Type_def \<phi>NatRound_def by simp
 
 lemma
   \<open>Inhabited (x \<Ztypecolon> \<nat>\<^sup>r[b]) \<longleftrightarrow> True\<close>
   unfolding Inhabited_def by (auto simp add: \<phi>expns)
 
-lemma [\<phi>reason for \<open>\<phi>Zero (T_int.mk ?b) \<nat>\<^sup>r[?b] ?z\<close>]:
-  "\<phi>Zero (T_int.mk b) (\<nat>\<^sup>r[b]) 0"
+lemma [\<phi>reason for \<open>\<phi>Zero (int.mk ?b) \<nat>\<^sup>r[?b] ?z\<close>]:
+  "\<phi>Zero (int.mk b) (\<nat>\<^sup>r[b]) 0"
   unfolding \<phi>Zero_def by (simp add: \<phi>expns)
 
 lemma \<phi>NatRound_semty[\<phi>reason for \<open>\<phi>SemType (?x \<Ztypecolon> \<nat>\<^sup>r[?b]) ?ty\<close>]:
-  \<open>\<phi>SemType (x \<Ztypecolon> \<nat>\<^sup>r[b]) (\<tau>Int b)\<close>
+  \<open>\<phi>SemType (x \<Ztypecolon> \<nat>\<^sup>r[b]) (int b)\<close>
   unfolding \<phi>SemType_def subset_iff by (simp add: \<phi>expns)
 
 subsubsection \<open>Integer in the normal sense\<close>
@@ -166,11 +174,11 @@ subsubsection \<open>Integer in the normal sense\<close>
 
 definition \<phi>Int :: "nat \<Rightarrow> ('VAL, int) \<phi>" ("\<int>[_]")
   where "\<phi>Int b x =(if x < 2^(b - 1) \<and> -(2^(b-1)) \<le> x \<and> (b = 0 \<longrightarrow> x = 0)
-                    then { V_int.mk (b, (if x \<ge> 0 then nat x else nat (2^b + x))) }
+                    then { V.Int.mk (b, (if x \<ge> 0 then nat x else nat (2^b + x))) }
                     else {})"
 
 lemma \<phi>Int_expn[\<phi>expns]:
-  "p \<in> (x \<Ztypecolon> \<int>[b]) \<longleftrightarrow> p = V_int.mk (b, (if x \<ge> 0 then nat x else nat (2^b + x)))
+  "p \<in> (x \<Ztypecolon> \<int>[b]) \<longleftrightarrow> p = V.Int.mk (b, (if x \<ge> 0 then nat x else nat (2^b + x)))
                       \<and> x < 2^(b - 1) \<and> -(2^(b-1)) \<le> x \<and> (b = 0 \<longrightarrow> x = 0)"
   unfolding \<phi>Type_def by (simp add: \<phi>Int_def)
 
@@ -186,12 +194,12 @@ lemma [\<phi>reason for \<open>\<phi>Equal \<int>[b] ?c ?eq\<close>]:
     "\<phi>Equal \<int>[b] (\<lambda>x y. True) (=)"
   unfolding \<phi>Equal_def by (cases b) (auto simp add: \<phi>expns eq_nat_nat_iff)
 
-lemma [\<phi>reason for \<open>\<phi>Zero (T_int.mk ?b) \<int>[?b] ?x\<close>]:
-    "\<phi>Zero (T_int.mk b) \<int>[b] 0"
+lemma [\<phi>reason for \<open>\<phi>Zero (int.mk ?b) \<int>[?b] ?x\<close>]:
+    "\<phi>Zero (int.mk b) \<int>[b] 0"
   unfolding \<phi>Zero_def by (simp add: \<phi>expns)
 
 lemma \<phi>Int_semty[\<phi>reason for \<open>\<phi>SemType (?x \<Ztypecolon> \<int>[?b]) ?ty\<close>]:
-  \<open>\<phi>SemType (x \<Ztypecolon> \<int>[b]) (\<tau>Int b)\<close>
+  \<open>\<phi>SemType (x \<Ztypecolon> \<int>[b]) (int b)\<close>
   unfolding \<phi>SemType_def subset_iff
   by (simp add: \<phi>expns Big_def) (smt (verit, ccfv_SIG) diff_le_self power_increasing_iff)
 
@@ -204,7 +212,7 @@ lemma subty_Z_N[\<phi>overload nat]:
   by (smt (verit, del_insts) diff_less less_numeral_extra(1) power_strict_increasing_iff)
 
 lemma subty_N_Z[\<phi>overload int]:
-  "\<^bold>p\<^bold>r\<^bold>e\<^bold>m\<^bold>i\<^bold>s\<^bold>e x < 2^(b - 1) \<Longrightarrow> x \<Ztypecolon> \<nat>[b] \<^bold>i\<^bold>m\<^bold>p\<^bold>l\<^bold>i\<^bold>e\<^bold>s int x \<Ztypecolon> \<int>[b]"
+  "\<^bold>p\<^bold>r\<^bold>e\<^bold>m\<^bold>i\<^bold>s\<^bold>e x < 2^(b - 1) \<Longrightarrow> x \<Ztypecolon> \<nat>[b] \<^bold>i\<^bold>m\<^bold>p\<^bold>l\<^bold>i\<^bold>e\<^bold>s Int.int x \<Ztypecolon> \<int>[b]"
   unfolding Imply_def Premise_def apply (simp add: \<phi>expns Big_def del: One_nat_def)
   by (metis less_one linorder_le_cases neg_0_le_iff_le not_exp_less_eq_0_int of_nat_0_le_iff order_trans power_0)
 
@@ -219,10 +227,10 @@ subsubsection \<open>Boolean\<close>
 qed *)
 
 definition \<phi>Bool :: "('VAL, bool) \<phi>" ("\<bool>")
-  where "\<bool> x = { V_int.mk (1, (if x then 1 else 0)) }"
+  where "\<bool> x = { V.Int.mk (1, (if x then 1 else 0)) }"
 
 lemma \<phi>Bool_expn[\<phi>expns]:
-  " p \<in> (x \<Ztypecolon> \<bool>) \<longleftrightarrow> p = V_int.mk (1, (if x then 1 else 0))"
+  " p \<in> (x \<Ztypecolon> \<bool>) \<longleftrightarrow> p = V.Int.mk (1, (if x then 1 else 0))"
   unfolding \<phi>Type_def \<phi>Bool_def by simp
 
 lemma \<phi>Bool_inhabited[\<phi>inhabitance_rule, elim!]:
@@ -232,12 +240,12 @@ lemma \<phi>Bool_eqcmp[\<phi>reason for \<open>\<phi>Equal \<bool> ?c ?eq\<close
   "\<phi>Equal \<bool> (\<lambda>x y. True) (=)"
   unfolding \<phi>Equal_def by (simp add: \<phi>expns)
 
-lemma \<phi>Bool_zero[\<phi>reason for \<open>\<phi>Zero (\<tau>Int 1) \<bool> ?z\<close>]:
-  "\<phi>Zero (\<tau>Int 1) \<bool> False"
+lemma \<phi>Bool_zero[\<phi>reason for \<open>\<phi>Zero (int 1) \<bool> ?z\<close>]:
+  "\<phi>Zero (int 1) \<bool> False"
   unfolding \<phi>Zero_def by (simp add: \<phi>expns)
 
 lemma \<phi>Bool_semty[\<phi>reason for \<open>\<phi>SemType (?x \<Ztypecolon> \<bool>) ?ty\<close>]:
-  \<open>\<phi>SemType (x \<Ztypecolon> \<bool>) (\<tau>Int 1)\<close>
+  \<open>\<phi>SemType (x \<Ztypecolon> \<bool>) (int 1)\<close>
   unfolding \<phi>SemType_def subset_iff
   by (simp add: \<phi>expns Big_def)
 
@@ -381,20 +389,20 @@ subsection \<open>Arithmetic Operations\<close>
 subsubsection \<open>Integer arithmetic\<close>
 
 definition op_const_int :: "nat \<Rightarrow> nat \<Rightarrow> ('VAL,'VAL,'RES_N,'RES) proc"
-  where "op_const_int bits const = Return (sem_value (V_int.mk (bits,const)))"
+  where "op_const_int bits const = Return (sem_value (V.Int.mk (bits,const)))"
 
 (* definition op_const_size_t :: "nat \<Rightarrow> ('VAL,'VAL,'RES_N,'RES) proc"
   where "op_const_size_t c = \<phi>M_assume (c < 2 ^ addrspace_bits)
-                          \<ggreater> Return (sem_value (V_int.mk (addrspace_bits,c)))"
+                          \<ggreater> Return (sem_value (V.Int.mk (addrspace_bits,c)))"
   \<comment> \<open> `op_const_size_t` checks the overflow during the compilation towards certain decided platform.  \<close>
 *)
 
 definition op_add :: "nat \<Rightarrow> ('VAL \<times> 'VAL, 'VAL, 'VAL, 'RES_N, 'RES) proc'"
   where "op_add bits =
       \<phi>M_caseV (\<lambda>vb va.
-      \<phi>M_getV (\<tau>Int bits) (snd o V_int.dest) vb (\<lambda>val_b.
-      \<phi>M_getV (\<tau>Int bits) (snd o V_int.dest) va (\<lambda>val_a.
-      Return (sem_value (V_int.mk (bits, ((val_a + val_b) mod 2^bits))))
+      \<phi>M_getV (int bits) (snd o V.Int.dest) vb (\<lambda>val_b.
+      \<phi>M_getV (int bits) (snd o V.Int.dest) va (\<lambda>val_a.
+      Return (sem_value (V.Int.mk (bits, ((val_a + val_b) mod 2^bits))))
   )))"
 
 
@@ -415,80 +423,80 @@ definition op_add :: "nat \<Rightarrow> ('VAL \<times> 'VAL, 'VAL, 'VAL, 'RES_N,
 definition op_sub :: "nat \<Rightarrow> ('VAL \<times> 'VAL, 'VAL, 'VAL, 'RES_N, 'RES) proc'"
   where "op_sub bits =
       \<phi>M_caseV (\<lambda>va vb.
-      \<phi>M_getV (\<tau>Int bits) (snd o V_int.dest) va (\<lambda>val_a.
-      \<phi>M_getV (\<tau>Int bits) (snd o V_int.dest) vb (\<lambda>val_b.
-      Return (sem_value (V_int.mk (bits, ((2^bits + val_b - val_a) mod 2^bits))))
+      \<phi>M_getV (int bits) (snd o V.Int.dest) va (\<lambda>val_a.
+      \<phi>M_getV (int bits) (snd o V.Int.dest) vb (\<lambda>val_b.
+      Return (sem_value (V.Int.mk (bits, ((2^bits + val_b - val_a) mod 2^bits))))
   )))"
 
 definition op_umul :: "nat \<Rightarrow> ('VAL \<times> 'VAL, 'VAL, 'VAL, 'RES_N, 'RES) proc'"
   where "op_umul bits =
       \<phi>M_caseV (\<lambda>va vb.
-      \<phi>M_getV (\<tau>Int bits) (snd o V_int.dest) va (\<lambda>val_a.
-      \<phi>M_getV (\<tau>Int bits) (snd o V_int.dest) vb (\<lambda>val_b.
-      Return (sem_value (V_int.mk (bits, ((val_b * val_a) mod 2^bits))))
+      \<phi>M_getV (int bits) (snd o V.Int.dest) va (\<lambda>val_a.
+      \<phi>M_getV (int bits) (snd o V.Int.dest) vb (\<lambda>val_b.
+      Return (sem_value (V.Int.mk (bits, ((val_b * val_a) mod 2^bits))))
   )))"
 
 definition op_udiv :: "nat \<Rightarrow> ('VAL \<times> 'VAL, 'VAL, 'VAL, 'RES_N, 'RES) proc'"
   where "op_udiv bits =
       \<phi>M_caseV (\<lambda>va vb.
-      \<phi>M_getV (\<tau>Int bits) (snd o V_int.dest) va (\<lambda>val_a.
-      \<phi>M_getV (\<tau>Int bits) (snd o V_int.dest) vb (\<lambda>val_b.
-      Return (sem_value (V_int.mk (bits, (val_b div val_a))))
+      \<phi>M_getV (int bits) (snd o V.Int.dest) va (\<lambda>val_a.
+      \<phi>M_getV (int bits) (snd o V.Int.dest) vb (\<lambda>val_b.
+      Return (sem_value (V.Int.mk (bits, (val_b div val_a))))
   )))"
 
 definition op_lshr :: "nat \<Rightarrow> nat \<Rightarrow> ('VAL \<times> 'VAL, 'VAL, 'VAL, 'RES_N, 'RES) proc'"
   where "op_lshr b_b b_a =
       \<phi>M_caseV (\<lambda>va vb.
-      \<phi>M_getV (\<tau>Int b_a) (snd o V_int.dest) va (\<lambda>val_a.
-      \<phi>M_getV (\<tau>Int b_b) (snd o V_int.dest) vb (\<lambda>val_b.
-      Return (sem_value (V_int.mk (b_b, (val_b div 2 ^ val_a))))
+      \<phi>M_getV (int b_a) (snd o V.Int.dest) va (\<lambda>val_a.
+      \<phi>M_getV (int b_b) (snd o V.Int.dest) vb (\<lambda>val_b.
+      Return (sem_value (V.Int.mk (b_b, (val_b div 2 ^ val_a))))
   )))"
 
 definition op_lshl :: "nat \<Rightarrow> nat \<Rightarrow> ('VAL \<times> 'VAL, 'VAL, 'VAL, 'RES_N, 'RES) proc'"
   where "op_lshl b_b b_a =
       \<phi>M_caseV (\<lambda>va vb.
-      \<phi>M_getV (\<tau>Int b_a) (snd o V_int.dest) va (\<lambda>val_a.
-      \<phi>M_getV (\<tau>Int b_b) (snd o V_int.dest) vb (\<lambda>val_b.
-      Return (sem_value (V_int.mk (b_b, (val_b * 2 ^ val_a))))
+      \<phi>M_getV (int b_a) (snd o V.Int.dest) va (\<lambda>val_a.
+      \<phi>M_getV (int b_b) (snd o V.Int.dest) vb (\<lambda>val_b.
+      Return (sem_value (V.Int.mk (b_b, (val_b * 2 ^ val_a))))
   )))"
 
 definition op_lt :: "nat \<Rightarrow> ('VAL \<times> 'VAL, 'VAL,'VAL,'RES_N,'RES) proc'"
   where "op_lt bits =
       \<phi>M_caseV (\<lambda>va vb.
-      \<phi>M_getV (\<tau>Int bits) (snd o V_int.dest) va (\<lambda>val_a.
-      \<phi>M_getV (\<tau>Int bits) (snd o V_int.dest) vb (\<lambda>val_b.
-      Return (sem_value (V_int.mk (1, (if val_b < val_a then 1 else 0))))
+      \<phi>M_getV (int bits) (snd o V.Int.dest) va (\<lambda>val_a.
+      \<phi>M_getV (int bits) (snd o V.Int.dest) vb (\<lambda>val_b.
+      Return (sem_value (V.Int.mk (1, (if val_b < val_a then 1 else 0))))
   )))"
 
 definition op_le :: "nat \<Rightarrow> ('VAL \<times> 'VAL, 'VAL,'VAL,'RES_N,'RES) proc'"
   where "op_le bits =
       \<phi>M_caseV (\<lambda>va vb.
-      \<phi>M_getV (\<tau>Int bits) (snd o V_int.dest) va (\<lambda>val_a.
-      \<phi>M_getV (\<tau>Int bits) (snd o V_int.dest) vb (\<lambda>val_b.
-      Return (sem_value (V_int.mk (1, (if val_b \<le> val_a then 1 else 0))))
+      \<phi>M_getV (int bits) (snd o V.Int.dest) va (\<lambda>val_a.
+      \<phi>M_getV (int bits) (snd o V.Int.dest) vb (\<lambda>val_b.
+      Return (sem_value (V.Int.mk (1, (if val_b \<le> val_a then 1 else 0))))
   )))"
 
 
 definition op_not :: "('VAL, 'VAL,'VAL,'RES_N,'RES) proc'"
   where "op_not v =
-    \<phi>M_getV (\<tau>Int 1) (snd o V_int.dest) v (\<lambda>v.
-    Return (sem_value (V_int.mk (1, 1 - v)))
+    \<phi>M_getV (int 1) (snd o V.Int.dest) v (\<lambda>v.
+    Return (sem_value (V.Int.mk (1, 1 - v)))
   )"
 
 definition op_and :: "('VAL \<times> 'VAL, 'VAL,'VAL,'RES_N,'RES) proc'"
   where "op_and =
     \<phi>M_caseV (\<lambda>va vb.
-    \<phi>M_getV (\<tau>Int 1) (snd o V_int.dest) va (\<lambda>v.
-    \<phi>M_getV (\<tau>Int 1) (snd o V_int.dest) vb (\<lambda>u.
-    Return (sem_value (V_int.mk (1, v+u-1)))
+    \<phi>M_getV (int 1) (snd o V.Int.dest) va (\<lambda>v.
+    \<phi>M_getV (int 1) (snd o V.Int.dest) vb (\<lambda>u.
+    Return (sem_value (V.Int.mk (1, v+u-1)))
   )))"
 
 definition op_or :: "('VAL \<times> 'VAL, 'VAL,'VAL,'RES_N,'RES) proc'"
   where "op_or =
     \<phi>M_caseV (\<lambda>va vb.
-    \<phi>M_getV (\<tau>Int 1) (snd o V_int.dest) va (\<lambda>v.
-    \<phi>M_getV (\<tau>Int 1) (snd o V_int.dest) vb (\<lambda>u.
-    Return (sem_value (V_int.mk (1, min 1 (v+u))))
+    \<phi>M_getV (int 1) (snd o V.Int.dest) va (\<lambda>v.
+    \<phi>M_getV (int 1) (snd o V.Int.dest) vb (\<lambda>u.
+    Return (sem_value (V.Int.mk (1, min 1 (v+u))))
   )))"
 
 definition op_equal :: "'TY \<Rightarrow> ('VAL \<times> 'VAL, 'VAL,'VAL,'RES_N,'RES) proc'"
@@ -497,7 +505,7 @@ definition op_equal :: "'TY \<Rightarrow> ('VAL \<times> 'VAL, 'VAL,'VAL,'RES_N,
     \<phi>M_getV TY id va (\<lambda>v.
     \<phi>M_getV TY id vb (\<lambda>u.
     (\<lambda>res. \<phi>M_assert (Can_EqCompare res u v) res) \<ggreater>
-    Return (sem_value (V_int.mk (1, (if EqCompare u v then 1 else 0))))
+    Return (sem_value (V.Int.mk (1, (if EqCompare u v then 1 else 0))))
 )))"
 
 
@@ -571,7 +579,7 @@ lemma (in \<phi>min) op_var_scope':
   apply (cases rawv; simp, rule, simp add: \<phi>expns)
   apply (clarsimp simp add: \<phi>expns \<phi>Procedure_\<phi>Res_Spec simp del: set_mult_expn del: subsetI)
   subgoal for r res c
-  apply (rule R_var.\<phi>R_allocate_res_entry[where R="(\<I> INTERP (r * c))"])
+  apply (rule R_var.\<phi>R_allocate_res_entry[where R="(\<I> F.INTERP (r * c))"])
      apply (clarsimp) using finite_map_freshness infinite_varname apply blast
       apply (clarsimp)
 
@@ -579,9 +587,9 @@ lemma (in \<phi>min) op_var_scope':
   subgoal premises prems for k res'
     apply (rule prems(2)[THEN spec[where x=r], THEN spec[where x=res'],
                 simplified prems, simplified, THEN mp])
-    apply (rule exI[where x=\<open>c * FIC_var.mk (1(k \<mapsto> v))\<close>])
+    apply (rule exI[where x=\<open>c * F.FIC_var.mk (1(k \<mapsto> v))\<close>])
     apply (simp add: \<phi>expns prems)
-    by (smt (verit, ccfv_threshold) FIC_var.expand FIC_var.sep_disj_fiction Fic_Space_Un Fic_Space_m \<phi>Res_Spec_mult_homo prems(5) prems(6) prems(7) prems(8) prems(9) sep_disj_multD2 sep_disj_multI2 sep_mult_assoc')
+    by (smt (verit, ccfv_threshold) FIC_var.expand FIC_var.sep_disj_fiction Fic_Space_Un F.Fic_Space_m \<phi>Res_Spec_mult_homo prems(5) prems(6) prems(7) prems(8) prems(9) sep_disj_multD2 sep_disj_multI2 sep_mult_assoc')
   . .
 
 
@@ -601,7 +609,7 @@ paragraph \<open>Non-Branching Selection\<close>
 definition op_sel :: "'TY \<Rightarrow> ('VAL \<times> 'VAL \<times> 'VAL, 'VAL,'VAL,'RES_N,'RES) proc'"
   where "op_sel TY =
     \<phi>M_caseV (\<lambda>vc. \<phi>M_caseV (\<lambda>va vb.
-    \<phi>M_getV (\<tau>Int 1) V_int.dest vc (\<lambda>c.
+    \<phi>M_getV (int 1) V.Int.dest vc (\<lambda>c.
     \<phi>M_getV TY id va (\<lambda>a.
     \<phi>M_getV TY id vb (\<lambda>b.
     Return (sem_value (if snd c = 1 then b else a)))))))"
@@ -612,20 +620,20 @@ definition op_if :: "('ret,'VAL,'RES_N,'RES) proc
                   \<Rightarrow> ('ret,'VAL,'RES_N,'RES) proc
                   \<Rightarrow> ('VAL,'ret,'VAL,'RES_N,'RES) proc'"
   where "op_if brT brF v =
-    \<phi>M_getV (\<tau>Int 1) V_int.dest v (\<lambda>c. (if snd c = 1 then brT else brF))"
+    \<phi>M_getV (int 1) V.Int.dest v (\<lambda>c. (if snd c = 1 then brT else brF))"
 
 paragraph \<open>While Loop\<close>
 
 inductive SemDoWhile :: "('VAL,'VAL,'RES_N,'RES) proc \<Rightarrow> ('RES_N \<Rightarrow> 'RES) \<Rightarrow> (unit,'VAL,'RES_N,'RES) state \<Rightarrow> bool" where
-  "Success (sem_value (V_int.mk (1,0))) res \<in> f s \<Longrightarrow> SemDoWhile f s (Success (sem_value ()) res)"
-| "Success (sem_value (V_int.mk (1,1))) res \<in> f s \<Longrightarrow> SemDoWhile f res s'' \<Longrightarrow> SemDoWhile f s s''"
+  "Success (sem_value (V.Int.mk (1,0))) res \<in> f s \<Longrightarrow> SemDoWhile f s (Success (sem_value ()) res)"
+| "Success (sem_value (V.Int.mk (1,1))) res \<in> f s \<Longrightarrow> SemDoWhile f res s'' \<Longrightarrow> SemDoWhile f s s''"
 | "Exception v e \<in> f s \<Longrightarrow> SemDoWhile f s (Exception v e)"
 | "PartialCorrect \<in> f s \<Longrightarrow> SemDoWhile f s PartialCorrect"
 | "Invalid \<in> f s \<Longrightarrow> SemDoWhile f s Invalid"
 
-lemma "\<nexists> y. SemDoWhile ((\<lambda>res. Return (sem_value (V_int.mk (1,1))) res)::('VAL,'VAL,'RES_N,'RES) proc) res y"
+lemma "\<nexists> y. SemDoWhile ((\<lambda>res. Return (sem_value (V.Int.mk (1,1))) res)::('VAL,'VAL,'RES_N,'RES) proc) res y"
   apply rule apply (elim exE) subgoal for y
-    apply (induct "((\<lambda>res. Return (sem_value (V_int.mk (1,1))) (res::'RES_N \<Rightarrow> 'RES))::('VAL,'VAL,'RES_N,'RES) proc)" res y
+    apply (induct "((\<lambda>res. Return (sem_value (V.Int.mk (1,1))) (res::'RES_N \<Rightarrow> 'RES))::('VAL,'VAL,'RES_N,'RES) proc)" res y
            rule: SemDoWhile.induct)
        apply (simp_all add: Return_def det_lift_def) . .
 
