Phi_System/PhiSem/Phi_Aggregate.thy
@@ -1,0 +1,417 @@
+theory Phi_Aggregate
+  imports PhiSem_Min
+begin
+
+section \<open>Semantics\<close>
+
+subsection \<open>Models\<close>
+
+subsubsection \<open>Type\<close>
+
+virtual_datatype aggregate_ty = \<phi>min_ty +
+  tup     :: \<open>'self list\<close>
+  array   :: \<open>'self \<times> nat\<close>
+
+context aggregate_ty begin
+
+abbreviation \<open>tup \<equiv> tup.mk\<close>
+abbreviation \<open>array N T \<equiv> array.mk (T,N)\<close>
+
+definition \<open>length_\<tau>Array T = (@N. \<exists>any. T = array N any)\<close>
+abbreviation \<open>is_\<tau>Array T t \<equiv> (\<exists>N. t = array N T)\<close>
+
+lemma length_\<tau>Array[simp]:
+  \<open>length_\<tau>Array (array N T) = N\<close>
+  unfolding length_\<tau>Array_def
+  by blast
+
+end
+
+subsubsection \<open>Value\<close>
+
+virtual_datatype 'TY aggregate_val :: "nonsepable_semigroup" = 'TY \<phi>min_val +
+  V_tup    :: \<open>'self list\<close>
+  V_array   :: \<open>'TY \<times> 'self list\<close>
+
+
+subsection \<open>Semantics\<close>
+
+datatype ('TY,'VAL) \<I>\<D>\<X> = mk_\<I>\<D>\<X>
+  (valid_idx_step: \<open>'TY \<Rightarrow> nat \<Rightarrow> bool\<close>)
+  (idx_step_type: \<open>nat \<Rightarrow> 'TY \<Rightarrow> 'TY\<close>)
+  (idx_step_value: \<open>nat \<Rightarrow> 'VAL \<Rightarrow> 'VAL\<close>)
+  (idx_step_mod_value: \<open>nat \<Rightarrow> ('VAL \<Rightarrow> 'VAL) \<Rightarrow> 'VAL \<Rightarrow> 'VAL\<close>)
+  (idx_step_offset: \<open>'TY \<Rightarrow> nat \<Rightarrow> nat\<close>)
+  (type_measure: \<open>'TY \<Rightarrow> nat\<close>)
+
+locale aggregate =
+  aggregate_ty where CONS_OF   = TY_CONS_OF
+            and TYPE'NAME = \<open>TYPE('TY_N)\<close>
+            and TYPE'REP  = \<open>TYPE('TY)\<close>
++ aggregate_val where CONS_OF   = VAL_CONS_OF
+            and TYPE'TY   = \<open>TYPE('TY)\<close>
+            and TYPE'NAME = \<open>TYPE('VAL_N)\<close>
+            and TYPE'REP  = \<open>TYPE('VAL::nonsepable_semigroup)\<close>
++ \<phi>min where TYPES = \<open>TYPE(('TY_N \<Rightarrow> 'TY)
+                  \<times> ('VAL_N \<Rightarrow> 'VAL::nonsepable_semigroup)
+                  \<times> ('RES_N \<Rightarrow> 'RES::sep_algebra)
+                  \<times> ('FIC_N \<Rightarrow> 'FIC::sep_algebra))\<close>
++ fixes TYPES :: \<open>(('TY_N \<Rightarrow> 'TY) \<times> ('VAL_N => 'VAL) \<times> ('RES_N => 'RES) \<times> ('FIC_N \<Rightarrow> 'FIC)) itself\<close>
+
+fixes \<I>\<D>\<X> :: \<open>('TY,'VAL) \<I>\<D>\<X>\<close>
+
+assumes WT_tup[simp]: \<open>Well_Type (\<tau>Tuple ts)  = { V_tup.mk vs       |vs. list_all2 (\<lambda> t v. v \<in> Well_Type t) ts vs }\<close>
+  and   WT_arr[simp]: \<open>Well_Type (\<tau>Array n t) = { V_array.mk (t,vs) |vs. length vs = n \<and> list_all (\<lambda>v. v \<in> Well_Type t) vs \<and> Valid_Type t }\<close>
+
+assumes zero_tup[simp]: \<open>Zero (T_tup.mk Ts)     = map_option V_tup.mk (those (map Zero Ts))\<close>
+  and   zero_arr[simp]: \<open>Zero (T_array.mk (T,N))=
+            map_option (\<lambda>z. V_array.mk (T, replicate N z)) (Zero T)\<close>
+
+
+assumes V_tup_mult: \<open>V_tup.mk t1 * V_tup.mk t2 = V_tup.mk (t1 @ t2)\<close>
+    and   idx_step_type_measure: \<open>valid_idx_step \<I>\<D>\<X> T i
+                              \<Longrightarrow> type_measure \<I>\<D>\<X> (idx_step_type \<I>\<D>\<X> i T) < type_measure \<I>\<D>\<X> T\<close>
+    and   idx_step_type_tup  : \<open>i < length tys \<Longrightarrow> idx_step_type \<I>\<D>\<X> i (\<tau>Tuple tys) = tys!i \<close>
+    and   idx_step_type_arr  : \<open>i \<le> N \<Longrightarrow> idx_step_type \<I>\<D>\<X> i (\<tau>Array N T) = T\<close>
+    and   valid_idx_step_tup : \<open>valid_idx_step \<I>\<D>\<X> (\<tau>Tuple tys) i \<longleftrightarrow> i < length tys\<close>
+    and   valid_idx_step_arr : \<open>valid_idx_step \<I>\<D>\<X> (\<tau>Array N T) i \<longleftrightarrow> i < N\<close>
+    and   idx_step_value_welltyp: \<open>valid_idx_step \<I>\<D>\<X> T i
+                               \<Longrightarrow> v \<in> Well_Type T
+                               \<Longrightarrow> idx_step_value \<I>\<D>\<X> i v \<in> Well_Type (idx_step_type \<I>\<D>\<X> i T)\<close>
+    and   idx_step_value_tup : \<open>idx_step_value \<I>\<D>\<X> i (V_tup.mk vs)   = vs!i\<close>
+    and   idx_step_value_arr : \<open>idx_step_value \<I>\<D>\<X> i (V_array.mk (T,vs)) = vs!i\<close>
+    and   idx_step_mod_value : \<open>valid_idx_step \<I>\<D>\<X> T i
+                            \<Longrightarrow> valid_idx_step \<I>\<D>\<X> T j
+                            \<Longrightarrow> v \<in> Well_Type T
+                            \<Longrightarrow> idx_step_value \<I>\<D>\<X> i (idx_step_mod_value \<I>\<D>\<X> j f v) =
+                                  (if i = j then f (idx_step_value \<I>\<D>\<X> j v) else idx_step_value \<I>\<D>\<X> i v) \<close>
+    and   idx_step_mod_value_welltyp: \<open>valid_idx_step \<I>\<D>\<X> T i
+                                   \<Longrightarrow> v \<in> Well_Type T
+                                   \<Longrightarrow> f (idx_step_value \<I>\<D>\<X> i v) \<in> Well_Type (idx_step_type \<I>\<D>\<X> i T)
+                                   \<Longrightarrow> idx_step_mod_value \<I>\<D>\<X> i f v \<in> Well_Type T\<close>
+    and   idx_step_mod_value_tup : \<open>idx_step_mod_value \<I>\<D>\<X> i f (V_tup.mk vs) = V_tup.mk (vs[i := f (vs!i)])\<close>
+    and   idx_step_mod_value_arr : \<open>idx_step_mod_value \<I>\<D>\<X> i f (V_array.mk (T,vs)) = V_array.mk (T,vs[i := f (vs!i)])\<close>
+    and   idx_step_offset_arr: \<open>idx_step_offset \<I>\<D>\<X> (\<tau>Array N T) i = i * MemObj_Size T\<close>
+begin
+thm distinct_names
+
+end
+
+print_locale aggregate
+
+typedecl TY_N
+typedecl TY
+typedecl VAL_N
+typedecl VAL
+typedecl FIC_N
+typedecl FIC
+typedecl RES_N
+typedecl RES
+
+axiomatization where VAL: \<open>OFCLASS(VAL, nonsepable_semigroup_class)\<close>
+and FIC: \<open>OFCLASS(FIC, sep_algebra_class)\<close>
+and RES: \<open>OFCLASS(RES, sep_algebra_class)\<close>
+
+setup \<open>Axclass.add_arity @{thm VAL}
+#> Axclass.add_arity @{thm FIC}
+#> Axclass.add_arity @{thm RES}
+\<close>
+
+print_locale aggregate
+
+axiomatization T_int :: "(TY_N, TY, nat) Virtual_Datatype.Field"
+and  T_tup :: "(TY_N, TY, TY list) Virtual_Datatype.Field"
+and  T_array :: "(TY_N, TY, TY \<times> nat) Virtual_Datatype.Field"
+and  V_int :: "(VAL_N, VAL, nat \<times> nat) Virtual_Datatype.Field"
+and  V_tup :: "(VAL_N, VAL, VAL list) Virtual_Datatype.Field"
+and  V_array :: "(VAL_N, VAL, TY \<times> VAL list) Virtual_Datatype.Field"
+and  INTERPRET :: "FIC_N \<Rightarrow> (FIC, RES_N \<Rightarrow> RES) interp"
+and  FIC_var :: "(FIC_N, FIC, varname \<Rightarrow> VAL option) Virtual_Datatype.Field"
+and  TY_CONS_OF :: "TY \<Rightarrow> TY_N"
+and  VAL_CONS_OF :: "VAL \<Rightarrow> VAL_N"
+and  Resource_Validator :: "RES_N \<Rightarrow> RES set"
+and  Well_Type :: "TY \<Rightarrow> VAL set"
+and  Can_EqCompare :: "(RES_N \<Rightarrow> RES) \<Rightarrow> VAL \<Rightarrow> VAL \<Rightarrow> bool"
+and  EqCompare :: "VAL \<Rightarrow> VAL \<Rightarrow> bool"
+and  Zero :: "TY \<Rightarrow> VAL option"
+and  R_var :: "(RES_N, RES, varname \<Rightarrow> VAL option) Virtual_Datatype.Field"
+and  \<I>\<D>\<X> :: "(TY, VAL) \<I>\<D>\<X>"
+where XXX: \<open>aggregate T_int T_tup T_array V_int V_tup V_array INTERPRET FIC_var TY_CONS_OF
+  VAL_CONS_OF Resource_Validator
+  Well_Type Can_EqCompare EqCompare Zero R_var \<I>\<D>\<X>\<close>
+
+interpretation ag: aggregate T_int T_tup T_array V_int V_tup V_array INTERPRET FIC_var TY_CONS_OF
+  VAL_CONS_OF Resource_Validator
+  Well_Type Can_EqCompare EqCompare Zero R_var _ \<I>\<D>\<X>
+  using XXX .
+
+
+lemma V_tup_mult_cons:
+  \<open>NO_MATCH vs ([]::'VAL list) \<Longrightarrow> V_tup.mk (v#vs) = V_tup.mk [v] * V_tup.mk vs\<close>
+  using V_tup_mult by simp
+
+abbreviation \<open>index_value \<equiv> fold (idx_step_value \<I>\<D>\<X>)\<close>
+abbreviation \<open>index_type  \<equiv> fold (idx_step_type \<I>\<D>\<X>)\<close>
+abbreviation \<open>index_mod_value \<equiv> foldr (idx_step_mod_value \<I>\<D>\<X>)\<close>
+
+primrec valid_index :: \<open>'TY \<Rightarrow> nat list \<Rightarrow> bool\<close>
+  where \<open>valid_index T [] \<longleftrightarrow> True\<close>
+      | \<open>valid_index T (i#idx) \<longleftrightarrow> valid_idx_step \<I>\<D>\<X> T i \<and> valid_index (idx_step_type \<I>\<D>\<X> i T) idx\<close>
+
+lemma valid_index_tail[simp]:
+  \<open>valid_index T (idx@[i]) \<longleftrightarrow> valid_index T idx \<and> valid_idx_step \<I>\<D>\<X> (index_type idx T) i\<close>
+  by (induct idx arbitrary: T; simp)
+
+lemma index_type_measure:
+  \<open>valid_index T idx \<Longrightarrow> idx \<noteq> [] \<Longrightarrow> type_measure \<I>\<D>\<X> (index_type idx T) < type_measure \<I>\<D>\<X> T\<close>
+  apply (induct idx arbitrary: T; simp)
+  by (metis dual_order.strict_trans fold_simps(1) idx_step_type_measure)
+
+lemma valid_index_cat: \<open>valid_index T (a@b) \<Longrightarrow> valid_index T a \<and> valid_index (index_type a T) b\<close>
+  by (induct a arbitrary: T; simp)
+
+lemma valid_index_cons: \<open>valid_index T [i] \<longleftrightarrow> valid_idx_step \<I>\<D>\<X> T i\<close> by simp
+
+lemma index_value_welltyp:
+  \<open>valid_index T idx \<Longrightarrow> v \<in> Well_Type T \<Longrightarrow> index_value idx v \<in> Well_Type (index_type idx T)\<close>
+  apply (induct idx arbitrary: v T; simp)
+  using idx_step_value_welltyp
+  by blast
+
+lemma index_mod_value_welltyp:
+   \<open>valid_index T idx
+\<Longrightarrow> v \<in> Well_Type T
+\<Longrightarrow> f (index_value idx v) \<in> Well_Type (index_type idx T)
+\<Longrightarrow> index_mod_value idx f v \<in> Well_Type T\<close>
+  apply (induct idx arbitrary: T v; simp)
+  using idx_step_mod_value_welltyp idx_step_value_welltyp by blast
+
+
+
+primrec index_offset :: \<open>'TY \<Rightarrow> nat list \<Rightarrow> nat\<close>
+  where \<open>index_offset T [] = 0\<close>
+      | \<open>index_offset T (i#idx) = idx_step_offset \<I>\<D>\<X> T i + index_offset (idx_step_type \<I>\<D>\<X> i T) idx\<close>
+
+lemma index_offset_tail[simp]:
+  \<open>index_offset T (idx@[i]) = index_offset T idx + idx_step_offset \<I>\<D>\<X> (index_type idx T) i\<close>
+  by (induct idx arbitrary: T; simp)
+
+lemma index_type_idem:
+  \<open>valid_index T idx \<Longrightarrow> index_type idx T = T \<longleftrightarrow> idx = []\<close>
+  apply (cases idx; simp; rule)
+  using index_type_measure
+  by (metis fold_simps(2) list.discI order_less_irrefl valid_index.simps(2))
+
+
+lemma Valid_Type_\<tau>Array[simp]:
+  \<open>Valid_Type (\<tau>Array n T) \<longleftrightarrow> Valid_Type T\<close>
+  apply (simp add: Inhabited_def)
+  apply (rule; clarsimp)
+
+lemma Valid_Type_\<tau>Tuple[simp]:
+  \<open>Valid_Type (\<tau>Tuple Ts) \<longleftrightarrow> list_all Valid_Type Ts\<close>
+  unfolding Inhabited_def
+  using Ball_set zero_well_typ by blas
+
+end
+
+
+section \<open>\<phi>Type\<close>
+
+context aggregate begin
+
+subsection \<open>Tuple\<close>
+
+subsubsection \<open>Empty Tuple\<close>
+
+definition EmptyTuple :: \<open>('VAL, unit) \<phi>\<close>
+  where \<open>EmptyTuple x = { V_tup.mk [] }\<close>
+
+lemma EmptyTuple_expn[\<phi>expns]:
+  \<open>p \<in> (x \<Ztypecolon> EmptyTuple) \<longleftrightarrow> p = V_tup.mk []\<close>
+  unfolding EmptyTuple_def \<phi>Type_def by simp
+
+subsubsection \<open>Field\<close>
+
+definition \<phi>Field :: "('VAL, 'a) \<phi> \<Rightarrow> ('VAL, 'a) \<phi>" ("\<clubsuit>")
+  where "\<phi>Field T x = { V_tup.mk [v] |v. v \<in> T x }"
+
+lemma \<phi>Field_expn[\<phi>expns]:
+  \<open>p \<in> (x \<Ztypecolon> \<phi>Field T) \<longleftrightarrow> (\<exists>v. p = V_tup.mk [v] \<and> v \<in> (x \<Ztypecolon> T))\<close>
+  unfolding \<phi>Field_def \<phi>Type_def by simp
+
+lemma \<phi>Field_inhabited[elim!,\<phi>inhabitance_rule]:
+  \<open>Inhabited (x \<Ztypecolon> \<clubsuit> T) \<Longrightarrow> (Inhabited (x \<Ztypecolon> T) \<Longrightarrow> C) \<Longrightarrow> C\<close>
+  unfolding Inhabited_def by (simp add: \<phi>expns)
+
+lemma EmptyTuple_reduce[simp]:
+  \<open>((a,()) \<Ztypecolon> \<clubsuit> T \<^emph> EmptyTuple) = (a \<Ztypecolon> \<clubsuit> T)\<close>
+  unfolding set_eq_iff apply (simp add: \<phi>expns V_tup_mult)
+  by (metis V_tup_mult append.left_neutral append_Cons)
+
+lemma \<phi>Field_zero  [\<phi>reason on \<open>\<phi>Zero (T_tup.mk [?ty]) (\<phi>Field ?T) ?x\<close>]:
+  \<open>\<phi>Zero ty T x \<Longrightarrow> \<phi>Zero (T_tup.mk [ty]) (\<clubsuit> T) x \<close>
+  unfolding \<phi>Zero_def by (simp add: \<phi>expns)
+
+lemma \<phi>Field_zeros [\<phi>reason on \<open>\<phi>Zero (T_tup.mk [?ty]) (\<phi>Field ?T) ?x\<close>]:
+  \<open>\<phi>Zero ty T x
+    \<Longrightarrow> \<phi>Zero (T_tup.mk tys) Ts xs
+    \<Longrightarrow> \<phi>Zero (T_tup.mk (ty#tys)) (\<clubsuit> T \<^emph> Ts) (x,xs) \<close>
+  unfolding \<phi>Zero_def
+  by (simp add: \<phi>expns V_tup_mult_cons) blast
+
+lemma \<phi>Field_semty[\<phi>reason on \<open>\<phi>SemType (?x \<Ztypecolon> \<clubsuit> ?T) ?ty\<close>]:
+  \<open>\<phi>SemType (x \<Ztypecolon> T) TY \<Longrightarrow> \<phi>SemType (x \<Ztypecolon> \<clubsuit> T) (\<tau>Tuple [TY])\<close>
+  unfolding \<phi>SemType_def subset_iff
+  by (clarsimp simp add: \<phi>expns)
+
+lemma \<phi>Field_semtsy[\<phi>reason on \<open>\<phi>SemType (?x \<Ztypecolon> \<clubsuit> ?T \<^emph> ?Ts) ?ty\<close>]:
+  \<open> \<phi>SemType (x \<Ztypecolon> T) TY
+\<Longrightarrow> \<phi>SemType (xs \<Ztypecolon> Ts) (\<tau>Tuple TYs)
+\<Longrightarrow> \<phi>SemType ((x,xs) \<Ztypecolon> (\<clubsuit> T \<^emph> Ts)) (\<tau>Tuple (TY#TYs))\<close>
+  unfolding \<phi>SemType_def subset_iff
+  apply (clarsimp simp add: \<phi>expns)
+  by (metis V_tup_mult append.left_neutral append_Cons list.rel_inject(2))
+
+subsubsection \<open>Helpers\<close>
+
+definition \<open>\<phi>Is_Tuple T x = { V_tup.mk vs |vs. V_tup.mk vs \<in> (x \<Ztypecolon> T) }\<close>
+
+lemma \<phi>Is_Tuple_expn[\<phi>expns]:
+  \<open>p \<in> (x \<Ztypecolon> \<phi>Is_Tuple T) \<longleftrightarrow> (\<exists>vs. p = V_tup.mk vs \<and> V_tup.mk vs \<in> (x \<Ztypecolon> T))\<close>
+  unfolding \<phi>Is_Tuple_def \<phi>Type_def by simp
+
+lemma \<phi>Is_Tuple_\<phi>Is_Tuple[simp]:
+  \<open>\<phi>Is_Tuple (\<phi>Is_Tuple T) = \<phi>Is_Tuple T\<close>
+  unfolding \<phi>Is_Tuple_def fun_eq_iff set_eq_iff \<phi>Type_def by simp
+
+
+lemma (in aggregate) \<phi>Is_Tuple_\<phi>Is_Tuple_more[simp]:
+  \<open>\<phi>Is_Tuple (\<clubsuit> A \<^emph> \<phi>Is_Tuple B) = (\<clubsuit> A \<^emph> \<phi>Is_Tuple B)\<close>
+  apply (rule \<phi>Type_eqI)
+  apply (clarsimp simp add: \<phi>expns, rule; clarify)
+  by (metis V_tup_mult)
+
+lemma (in aggregate) \<phi>Is_Tuple_Field[simp]:
+  \<open>\<phi>Is_Tuple (\<clubsuit> A) = \<clubsuit> A\<close>
+  by (rule \<phi>Type_eqI, clarsimp simp add: \<phi>expns, rule; clarify; blast)
+
+lemma (in aggregate) \<phi>Is_Tuple_EmptyTuple[simp]:
+  \<open>\<phi>Is_Tuple EmptyTuple = EmptyTuple\<close>
+  by (rule \<phi>Type_eqI, clarsimp simp add: \<phi>expns)
+
+
+
+subsection \<open>Array\<close>
+
+definition Array :: "nat \<Rightarrow> ('VAL, 'a) \<phi> \<Rightarrow> ('VAL, 'a list) \<phi>"
+  where \<open>Array N T = (\<lambda>l. { V_array.mk (TY,vs) |TY vs.
+    length l = N \<and> list_all2 (\<lambda>v x. v \<in> (x \<Ztypecolon> T)) vs l \<and> \<phi>\<phi>SemType T TY \<and> (\<exists>x. Inhabited (x \<Ztypecolon> T)) })\<close>
+
+lemma Array_expns[\<phi>expns]:
+  \<open>v \<in> (l \<Ztypecolon> Array N T) \<longleftrightarrow>
+    (\<exists> TY vs. length l = N \<and> v = V_array.mk (TY,vs) \<and> list_all2 (\<lambda>v x. v \<in> (x \<Ztypecolon> T)) vs l
+        \<and> \<phi>\<phi>SemType T TY \<and> (\<exists>x. Inhabited (x \<Ztypecolon> T)))\<close>
+  unfolding Array_def \<phi>Type_def by simp blast
+
+lemma Array_inhabited[\<phi>inhabitance_rule, elim!]:
+  \<open> Inhabited (l \<Ztypecolon> Array N T)
+\<Longrightarrow> (length l = N \<Longrightarrow>(\<And>i. i < length l \<Longrightarrow> Inhabited (l!i \<Ztypecolon> T)) \<Longrightarrow> C)
+\<Longrightarrow> C\<close>
+  unfolding Inhabited_def by (clarsimp simp add: \<phi>expns list_all2_conv_all_nth) blast
+
+lemma Array_semty[\<phi>reason on \<open>\<phi>SemType (?x \<Ztypecolon> Array ?N ?T) ?ty\<close>]:
+  \<open>(\<And>x. \<phi>SemType (x \<Ztypecolon> T) TY) \<Longrightarrow> \<phi>SemType (x \<Ztypecolon> Array N T) (\<tau>Array N TY)\<close>
+  apply (clarsimp simp add: \<phi>expns list_all_length list_all2_conv_all_nth \<phi>SemType_def subset_iff
+          Inhabited_def)
+  using Well_Type_unique by blast
+  
+lemma Array_zero[\<phi>reason on \<open>\<phi>Zero (\<tau>Array ?N ?TY) (Array ?N ?T) ?x\<close>]:
+  \<open>\<phi>Zero TY T zero \<Longrightarrow> \<phi>\<phi>SemType T TY \<Longrightarrow> \<phi>Zero (\<tau>Array N TY) (Array N T) (replicate N zero)\<close>
+  unfolding \<phi>Zero_def by (simp add: \<phi>expns list_all2_conv_all_nth Inhabited_def; blast)
+
+
+subsection \<open>Index to Fields of Structures\<close>
+
+definition \<phi>Index_getter :: \<open>nat list \<Rightarrow> ('VAL,'a) \<phi> \<Rightarrow> ('VAL,'b) \<phi> \<Rightarrow> ('a \<Rightarrow> 'b) \<Rightarrow> bool\<close>
+  where \<open>\<phi>Index_getter idx T U g \<longleftrightarrow> index_value idx \<in> (g \<Ztypecolon> T \<Rrightarrow> U)\<close>
+
+definition \<phi>Index_mapper :: \<open>nat list \<Rightarrow> ('VAL,'a) \<phi> \<Rightarrow> ('VAL,'b) \<phi> \<Rightarrow> (('b \<Rightarrow> 'b) \<Rightarrow> 'a \<Rightarrow> 'a) \<Rightarrow> bool\<close>
+  where \<open>\<phi>Index_mapper idx T U f \<longleftrightarrow> (\<forall>g g'. g \<in> (g' \<Ztypecolon> U \<Rrightarrow> U) \<longrightarrow> index_mod_value idx g \<in> (f g' \<Ztypecolon> T \<Rrightarrow> T))\<close>
+
+
+lemma idx_step_value_V_tup_suc:
+  \<open>idx_step_value \<I>\<D>\<X> (Suc i) (V_tup.mk (va # vs)) = idx_step_value \<I>\<D>\<X> i (V_tup.mk vs)\<close>
+  by (simp add: idx_step_value_tup)
+
+lemma idx_step_mod_value_V_tup_suc:
+  \<open>idx_step_mod_value \<I>\<D>\<X> (Suc i) g (V_tup.mk (va # vs)) = V_tup.mk [va] * idx_step_mod_value \<I>\<D>\<X> i g (V_tup.mk vs)\<close>
+  by (metis NO_MATCH_I V_tup_mult_cons idx_step_mod_value_tup list_update_code(3) nth_Cons_Suc)
+  
+
+
+
+lemma (in aggregate) \<phi>Index_getter_tup_suc:
+  \<open> \<phi>Index_getter (i # idx) X Y f
+\<Longrightarrow> \<phi>Index_getter (Suc i # idx) (\<clubsuit> T \<^emph> \<phi>Is_Tuple X) Y (f o snd)\<close>
+  unfolding \<phi>Index_getter_def
+  by (clarsimp simp add: \<phi>expns V_tup_mult idx_step_value_V_tup_suc)
+
+lemma (in aggregate) \<phi>Index_getter_tup_0:
+  \<open> \<phi>Index_getter idx X Y f
+\<Longrightarrow> \<phi>Index_getter (0 # idx) (\<clubsuit> X) Y f\<close>
+  unfolding \<phi>Index_getter_def
+  by (clarsimp simp add: \<phi>expns V_tup_mult idx_step_value_tup)
+
+lemma (in aggregate) \<phi>Index_getter_tup_0r:
+  \<open> \<phi>Index_getter idx X Y f
+\<Longrightarrow> \<phi>Index_getter (0 # idx) (\<clubsuit> X \<^emph> \<phi>Is_Tuple R) Y (f o fst)\<close>
+  unfolding \<phi>Index_getter_def
+  by (clarsimp simp add: \<phi>expns V_tup_mult idx_step_value_tup)
+
+lemma (in aggregate) \<phi>Index_getter_arr:
+  \<open> \<phi>Index_getter idx X Y f
+\<Longrightarrow> \<^bold>p\<^bold>r\<^bold>e\<^bold>m\<^bold>i\<^bold>s\<^bold>e i < N
+\<Longrightarrow> \<phi>Index_getter (i # idx) (Array N X) Y (\<lambda>l. f (l!i))\<close>
+  unfolding \<phi>Index_getter_def Premise_def
+  by (clarsimp simp add: \<phi>expns V_tup_mult idx_step_value_arr list_all2_conv_all_nth)
+
+
+
+lemma (in aggregate) \<phi>Index_mapper_tup_suc:
+  \<open> \<phi>Index_mapper (i # idx) X Y f
+\<Longrightarrow> \<phi>Index_mapper (Suc i # idx) (\<clubsuit> T \<^emph> \<phi>Is_Tuple X) Y (apsnd o f)\<close>
+  unfolding \<phi>Index_mapper_def
+  apply (clarsimp simp add: \<phi>expns V_tup_mult idx_step_mod_value_V_tup_suc)
+  by (metis idx_step_mod_value_tup)
+
+lemma (in aggregate) \<phi>Index_mapper_tup_0:
+  \<open> \<phi>Index_mapper idx X Y f
+\<Longrightarrow> \<phi>Index_mapper (0 # idx) (\<clubsuit> X) Y f\<close>
+  unfolding \<phi>Index_mapper_def
+  by (clarsimp simp add: \<phi>expns V_tup_mult idx_step_mod_value_tup)
+
+lemma (in aggregate) \<phi>Index_mapper_tup_0r:
+  \<open> \<phi>Index_mapper idx X Y f
+\<Longrightarrow> \<phi>Index_mapper (0 # idx) (\<clubsuit> X \<^emph> \<phi>Is_Tuple X) Y (apfst o f)\<close>
+  unfolding \<phi>Index_mapper_def
+  apply (clarsimp simp add: \<phi>expns V_tup_mult idx_step_mod_value_tup)
+  by (metis V_tup_mult append.left_neutral append_Cons)
+
+lemma (in aggregate) \<phi>Index_mapper_arr:
+  \<open> \<phi>Index_mapper idx X Y f
+\<Longrightarrow> \<^bold>p\<^bold>r\<^bold>e\<^bold>m\<^bold>i\<^bold>s\<^bold>e i < N
+\<Longrightarrow> \<phi>Index_mapper (i # idx) (Array N X) Y (\<lambda>g l. l[i := f g (l!i)])\<close>
+  unfolding \<phi>Index_mapper_def Premise_def
+  apply (clarsimp simp add: \<phi>expns V_tup_mult idx_step_mod_value_arr list_all2_conv_all_nth)
+  by (metis nth_list_update)
+
+
+
+end
+
+
+hide_const (open) valid_idx_step idx_step_type idx_step_value idx_step_mod_value idx_step_offset type_measure
+hide_const (open) \<I>\<D>\<X>
+
+end
